io/Compiler.Model2.Examples.fst
@@ -9,17 +9,17 @@ open FStar.List
 open Compiler.Model2
 
 (** Utils **)
-type source_arrow (arg:Type u#a) (res:Type u#b) (pre:arg -> trace -> Type0) (post:arg -> trace -> resexn res -> trace -> Type0) (fl:erased tflag) =
-  x:arg -> MIO (resexn res) fl (pre x) (post x)
+type source_arrow (mst:mst) (arg:Type u#a) (res:Type u#b) (pre:arg -> trace -> Type0) (post:arg -> trace -> resexn res -> trace -> Type0) (fl:erased tflag) =
+  x:arg -> MIO (resexn res) mst fl (pre x) (post x)
 
 type c1_post (#arg:Type u#a) (#res:Type u#b) (pre:arg -> trace -> Type0) (post:arg -> trace -> resexn res -> trace -> Type0) (pi:policy_spec) =
   squash (forall x h lt. pre x h /\ enforced_locally pi h lt ==> post x h (Inr Contract_failure) lt)
   
-type c2_post (#arg:Type u#a) (#res:Type u#b) (pre:arg -> trace -> Type0) (post:arg -> trace -> resexn res -> trace -> Type0) (pi:policy_spec) (dc:dc_typ arg (resexn res)) =
-  squash (forall x h lt r. pre x h /\ enforced_locally pi h lt /\ dc x h r lt ==> post x h r lt)
+type c2_post (#arg:Type u#a) (#res:Type u#b) (pre:arg -> trace -> Type0) (post:arg -> trace -> resexn res -> trace -> Type0) (pi:policy_spec) (idc:idc_typ arg (resexn res)) =
+  squash (forall x h lt r. pre x h /\ enforced_locally pi h lt /\ idc x h r lt ==> post x h r lt)
 
-type c1_pre (#arg:Type u#a) (#res:Type u#b) (pre:arg -> trace -> Type0) (post:arg -> trace -> resexn res -> trace -> Type0) (pi:policy_spec) (dc:dc_typ arg unit) =
-  squash (forall h x. dc x h () [] ==> pre x h)
+type c1_pre (#arg:Type u#a) (#res:Type u#b) (pre:arg -> trace -> Type0) (post:arg -> trace -> resexn res -> trace -> Type0) (pi:policy_spec) (idc:idc_typ arg unit) =
+  squash (forall h x. idc x h () [] ==> pre x h)
 
 type c2_pre (#arg:Type u#a) (#res:Type u#b) (pre:arg -> trace -> Type0) (post:arg -> trace -> resexn res -> trace -> Type0) (pi:policy_spec) =
   squash (forall x h lt r. pre x h /\ post x h r lt ==> enforced_locally pi h lt)
@@ -27,6 +27,10 @@ type c2_pre (#arg:Type u#a) (#res:Type u#b) (pre:arg -> trace -> Type0) (post:ar
 type stronger_pis (pi1:policy_spec) (pi2:policy_spec) =
   squash (forall h lt. enforced_locally pi1 h lt ==> enforced_locally pi2 h lt)
 
+let mst1 : mst = {
+  cst = list file_descr;
+  models = (fun s h -> forall fd. memP fd s <==> is_open fd h);
+}
 
 (** ** Testing **)
 (** *** Test 1 - FO **)
@@ -37,7 +41,7 @@ let test1_pi : policy_spec =
     | Openfile -> (arg <> "/etc/passwd")
     | _ -> True)
 
-let test1_phi : policy test1_pi =
+let test1_phi : policy mst1 test1_pi =
   fun h cmd arg -> 
     match cmd, arg with 
     | Openfile, s -> 
@@ -48,11 +52,11 @@ let test1_phi : policy test1_pi =
 let test1_pre = (fun (fd:file_descr) h -> b2t(is_open fd h))
 let test1_post = (fun (fd:file_descr) h (r:resexn unit) lt -> enforced_locally test1_pi h lt)
 
-type test1_pt = source_arrow file_descr unit test1_pre test1_post
+type test1_pt = source_arrow mst1 file_descr unit test1_pre test1_post
     
 let test1_pt_rc = (fun (fd:file_descr) h _ lt -> is_open fd h)
-let test1_pt_rcs : tree pck_dc = 
-  Node (| file_descr, unit, test1_pt_rc |) 
+let test1_pt_rcs : tree (pck_dc mst1) = 
+  Node (| file_descr, unit, test1_pt_rc, (fun fd s0 _ _ -> fd `List.mem` s0) |) 
     Leaf 
     Leaf
 
@@ -62,7 +66,7 @@ let test1_c1_pre = ()
 val test1_c2_pre : c2_pre test1_pre test1_post test1_pi
 let test1_c2_pre = ()
 
-let test1_pt_exportable (fl:erased tflag) : exportable (test1_pt fl) fl test1_pi test1_pt_rcs =
+let test1_pt_exportable (fl:erased tflag) : exportable (test1_pt fl) fl test1_pi mst1 test1_pt_rcs =
   exportable_arrow_pre_post_args
     _ _
     test1_pre
@@ -82,6 +86,7 @@ let test1_stronger_pis =
 
 [@@ (postprocess_with (fun () -> norm [delta_only [`%test1_pt; `%source_arrow; `%test1_pt_exportable]]; trefl ()))]
 let test1 : src_interface = {
+  mst = mst1;
   pi = test1_pi; phi = test1_phi;
 
   pt = test1_pt;
@@ -90,14 +95,15 @@ let test1 : src_interface = {
   pt_exportable = test1_pt_exportable;
 }
 
+#push-options "--compat_pre_core 1"
 val test1_prog : prog_src test1
-let test1_prog #fl fd : MIO (resexn unit) (fl+IOActions) (test1_pre fd) (test1_post fd) =
+let test1_prog #fl fd : MIO (resexn unit) mst1 (fl+IOActions) (test1_pre fd) (test1_post fd) =
   // weird behavior of F*
-  let r : mio_sig.res Close fd = static_cmd Ctx Close fd in
+  let r : (mio_sig mst1).res Close fd = static_cmd Ctx Close fd in
   r <: resexn unit
 
 val test1_ctx : ctx_src test1
-let test1_ctx #fl io_acts eff_rcs prog () : MIOpi int fl test1.pi = 
+let test1_ctx #fl io_acts eff_rcs prog () : MIOpi int fl test1.pi mst1 = 
   let fd = io_acts Openfile "/etc/passwd" in
   (match fd with
   | Inl fd -> let _ = prog fd in ()
@@ -105,7 +111,7 @@ let test1_ctx #fl io_acts eff_rcs prog () : MIOpi int fl test1.pi =
   0
 
 val test1_ctx_t : ctx_tgt (comp_int_src_tgt test1)
-let test1_ctx_t #fl io_acts prog () : MIOpi int fl test1.pi =
+let test1_ctx_t #fl io_acts prog () : MIOpi int fl test1.pi mst1 =
   let fd = io_acts Openfile "/etc/passwd" in
   (match fd with
   | Inl fd -> let _ = prog fd in ()
